plugins/Types/LTS/edu.toronto.cs.se.mmint.types.lts.operators/lean/common_meta.lean
@@ -1,5 +1,8 @@
-import system.io tactic justification
+import system.io tactic justification LTS property_catalogue.LTL.patterns
 open io list lean.parser tactic interactive.types
+
+open lean.parser (ident)
+
 
 meta def read {α : Type}
 (f : string)
@@ -25,7 +28,7 @@ meta def try_tactic_on_goal (tac: tactic unit)
 (goal : expr) : tactic bool := 
 set_goal goal >> tac >> is_solved
 
-meta def deconstruct_hyp (n : ℕ) : tactic unit := 
+meta def convert_to_premises (n : ℕ) : tactic unit := 
 do 
    (list.range n).mmap 
    (λ i, do 
@@ -33,51 +36,151 @@ do
    tactic.interactive.«have» h none ```(H ⟨%%(reflect i), dec_trivial⟩)),
    `[clear H, try {dsimp at *}]
 
-meta def new_str (s1 s2 : string) : tactic string := 
+namespace expr 
+
+meta def log_format (e : expr) : tactic string := 
+do 
+   e_fmt ← tactic_format_expr e,
+   pure e.to_string
+
+end expr 
+
+namespace string 
+
+meta def log (s1 s2 : string) : tactic string := 
 pure (s1 ++ s2)
 
+end string  
 
-meta def initialize (n : ℕ) (S : expr) : tactic string := 
+
+meta def analyze (n : ℕ) : tactic unit := 
 do  
-  let s : string := string.empty,
-  tactic.interactive.apply ``(property.deductive_of_justfd %%S),
-  e ←  tactic_format_expr S,
-  s ← new_str s ("apply property.deductive_of_justfd " ++ (format.to_string e) ++ ",\n"),
- `[rw property.justified],  s ← new_str s "rw property.justified,\n",
- `[simp], s ← new_str s "simp,\n",
- `[rw set.Inter], s ← new_str s "rw set.Inter,\n",
+  tactic.interactive.apply ``(property.deductive_of_justfd _),
+ `[rw property.justified], 
+ `[rw set.Inter], 
   x ← get_unused_name `x, H ← get_unused_name `H,
-  intro x,  s ← new_str s  "intro x,\n",
-  n_str ← pure (repr n),
- `[simp], s ← new_str s "simp,\n",
-  intro H, s ← new_str s  "intro H,\n",
-  deconstruct_hyp n,
-  s ← new_str s ("deconstruct_hyp " ++ n_str ++ ", \n"),
-  return s
+  intro x,  
+  intro H, 
+  `[simp at *],
+  convert_to_premises n,
+   `[repeat {rw sat at *}],
+   try `[simp at *]
 
 
-meta def by_induction (s : string) : tactic string := 
+
+meta def base_case (tgt : expr) : list expr → tactic string
+| [] := return string.empty
+| (h::t) := 
+  (infer_type h >>= unify tgt) >> 
+  (do `[exact %%h], h ← h.log_format, 
+  return h)
+  <|> base_case t
+
+
+meta def get_index_expr : list expr → tactic  expr
+| [] := failed
+| (h::t) := do 
+            h_t ← infer_type h,
+            nnat ← to_expr ``(ℕ),
+            unify nnat h_t >> 
+            return h <|> get_index_expr t
+            
+
+meta def inductive_case  : list expr → tactic (option string)
+| [] := return none
+| (h ::t) := do 
+       h_t ← infer_type h,
+       match h_t with 
+       | `(∀ i : ℕ, %%body) := 
+        (do 
+           ii ← local_context >>= get_index_expr,
+           let e := expr.mk_app h [ii],
+           `[apply %%e],
+           h ← h.log_format, ii ← ii.log_format,
+           return $ some h)
+         <|> inductive_case t
+       | _ := inductive_case t
+      end
+
+meta def debug (s : string): tactic (string × string) := 
+do 
+   tgt ← tactic.target,
+   match tgt with 
+   | `(%%path ⊨ %%e1) := 
+      match e1 with 
+      | `(formula.neg %%e2) := do  
+      let e3 : expr := expr.const `transitions_safe [],
+      let e4 : expr := expr.mk_app e3 [e2],
+      e2 ← tactic_format_expr e2,
+      e4 ← tactic_format_expr e4,
+      return $ ⟨s, to_string e4 ++ " " ++ to_string e2⟩
+      | _ := return ⟨s, string.empty⟩
+      end
+   |  _ :=    return ⟨s, string.empty⟩
+   end 
+
+meta def by_induction (s : string) : tactic (string × string) := 
 do
-   i ← get_unused_name `i,
-   intro i, s ← new_str s  "intro i,\n",
-   `[induction i with i IH],
-   s ← new_str s  "induction i with i IH,\n",
-   assumption,
-   s ← new_str s  "assumption,\n",
-   `[apply H2],
-    s ← new_str s  "apply H2,\n",
-   `[exact IH],
-   new_str s "exact IH"
+   analyze 2,
+   i ← get_unused_name `i, 
+   IH ← get_unused_name `IH,
+   `[repeat {rw sat at *}], 
+   intro i, 
+   `[induction i with i IH], -- fix this, logan!
+   s ← pure $ s.append  "by_induction,\n",
+   tgt ← target,
+   s' ← local_context >>= base_case tgt ,
+   s ← pure $ s.append  "base_case " ++ s' ++ ",\n",
+   ic_res ← local_context >>= inductive_case,
+   match ic_res with 
+   | none := debug s
+   | (some s'') := 
+   do
+   s ← pure $ s.append  "inductive_case " ++ s'' ++ ",\n",
+   tgt ← target,
+   local_context >>= base_case tgt ,
+   return ⟨s,string.empty⟩ 
+   end 
 
-meta def by_cases (s : string) : tactic string := 
+
+
+
+meta def match_hyps (s : string) : tactic string := 
 do  
    repeat1 (applyc `and.intro),
-   s ← new_str s "repeat {apply and.intro},\n",
+   s.log "repeat {apply and.intro},\n",
    `[repeat {assumption}],
-   new_str s "repeat {assumption}"
+   s.log "repeat {assumption}"
 
-meta def solve_hardcoded (n : ℕ) (S : expr) : tactic string := 
+
+meta def match_premises : tactic unit := 
+do  
+   repeat1 (applyc `and.intro), `[repeat {assumption}]
+
+
+
+open interactive (parse)
+
+meta def tactic.interactive.base_case (H : parse ident) : tactic unit := 
+do   
+   e ← get_local H,
+   tactic.exact e
+
+
+meta def tactic.interactive.inductive_case (H : parse ident) : tactic unit := 
+do   
+   e ← get_local H,
+    ii ← local_context >>= get_index_expr,
+           let e := expr.mk_app e [ii],
+         `[apply %%e],
+         `[assumption]
+
+meta def tactic.interactive.by_induction : tactic unit := 
 do 
-   s₁ ← initialize n S,
-   s₂ ← (by_induction s₁ <|> by_cases s₁ <|> return string.empty),
-   return s₂
+   analyze 2,
+   i ← get_unused_name `i, 
+   IH ← get_unused_name `IH,
+    `[repeat {rw sat at *}], 
+     try `[simp at *],
+    intro i, 
+   `[induction i with i IH] -- fix this, logan!
