plugins/Types/LTS/edu.toronto.cs.se.mmint.types.lts.operators/lean/property_catalogue/LTL/sat/precedes.lean
@@ -8,9 +8,6 @@ namespace precedes
 
 namespace globally
 
--- precedes.globally P S 
--- i.e. if S happens, P must happen first 
-
 
 -- Proof 1 : Because S never happens 
 lemma vacuous (P S : formula M) (π : path M) : 
@@ -19,10 +16,13 @@ lemma vacuous (P S : formula M) (π : path M) :
 
 -- Proof 2 : P precedes S because S can't happen before P
 
-lemma by_absent_before (P S : formula M) (π : path M) : 
- (sat (absent.before S P) π) ∧ 
- (sat (exist.globally P) π)  → 
-  sat (precedes.globally P S) π := 
+local notation π `⊨ `P := sat P π 
+
+variables (P Q R : formula M) (π : path M)
+
+lemma by_absent_before (P Q : formula M) (π : path M) : 
+ (π ⊨ absent.before Q P) ∧ (π ⊨ exist.globally P ) → 
+ (π ⊨ precedes.globally P Q)  := 
 begin 
  rintros ⟨H1,H2⟩,
  rw precedes.globally, 
@@ -34,16 +34,16 @@ end
 
 -- Proof 3 : P precedes R because P precedes Q and Q precedes R 
 
+
 lemma by_transitive (P Q R : formula M) (π : path M) : 
-    (sat (precedes.globally P Q) π ) ∧ 
-    (sat (precedes.globally Q R) π) → 
-    (sat (precedes.globally P R) π) := 
+    (π ⊨ precedes.globally P R) ∧ (π ⊨ precedes.globally R Q) → 
+    (π ⊨ precedes.globally P Q) := 
 begin
     rintros ⟨H1, H2⟩,
     cases H2, left, assumption,
     cases H1,
     cases H2 with k H2, replace H1 := (H1 k), replace H2:= H2.1, 
-    have := sat_em Q (π.drop k),replace this := this H2,
+    have := sat_em R (π.drop k),replace this := this H2,
     contradiction,
     rcases H1 with ⟨k,Hk1,Hk2⟩,
     rcases H2 with ⟨w, Hw1, Hw2⟩,
@@ -59,42 +59,41 @@ begin
     rw ← EM2, assumption,
     have : w < k, by omega,
     replace Hk2 := Hk2 w this,
-    have := sat_em Q (π.drop w),replace this := this Hw1,
+    have := sat_em R (π.drop w),replace this := this Hw1,
     contradiction,
 end 
 
-meta def solve_by_transitive (tok1 tok2 tok3: expr) (str : string): tactic string := 
+meta def solve_by_transitive (e₁ e₂ e₃ : expr) (s : string): tactic string := 
 do
-  tactic.interactive.apply ``(by_transitive %%tok1 _ %%tok2), 
-  t1 ← tactic_format_expr tok1,
-  t2 ← tactic_format_expr tok2,
-  t3 ← tactic_format_expr tok3,
-  new_str str $
-  "apply precedes.globally.by_transitive " ++ 
-  t1.to_string ++ " " ++ 
-  t3.to_string ++ " " ++ 
-  t2.to_string ++ ",\n"
+  tactic.interactive.apply ``(by_transitive %%e₁  %%e₂  %%e₃), 
+  e₁ ← tactic_format_expr e₁,
+    e₂ ← tactic_format_expr e₂,
+    e₃ ← tactic_format_expr e₃,
 
-meta def solve_by_absent_before (tok1 tok2 : expr) (str : string) : 
+  tactic.trace e₁,
+  return $  s.append $
+  "apply precedes.globally.by_transitive " ++ 
+  e₁.to_string  ++ " " ++ e₂.to_string  ++ " " ++ e₃.to_string  ++ ",\n"
+
+meta def solve_by_absent_before (e₁ e₂ : expr) (s : string) : 
 tactic string := 
 do  
-  tactic.interactive.apply ``(by_absent_before %%tok1 %%tok2),
-  t1 ← tactic_format_expr tok1,
-  t2 ← tactic_format_expr tok2,
-  new_str str $ 
+  tactic.interactive.apply ``(by_absent_before %%e₁ %%e₂),
+  e₁ ← e₁.log_format,
+  e₂ ← e₂.log_format,
+  s.log $ 
   "apply precedes.globally.by_absent_before " ++ 
-  t1.to_string ++ " " ++ 
-  t2.to_string ++ ",\n"
+  e₁ ++ " " ++ e₂ ++ ",\n"
 
-meta def solve (tok1 tok2 : expr) (str : string) : list expr → tactic string
+meta def solve (e₁  e₂ : expr) (s : string) : list expr → tactic string
 | [] :=  return string.empty
 | (h::t) := 
 do typ ← infer_type h,
    match typ with 
    | `(sat (precedes.globally _ %%new) _) := 
-       solve_by_transitive tok1 tok2 new str <|> solve t
+       solve_by_transitive e₁ e₂ new s <|> solve t
    | `(sat (absent.before _ _) _) := 
-      solve_by_absent_before tok1 tok2 str  <|> solve t 
+      solve_by_absent_before e₁ e₂ s  <|> solve t 
    | _ := solve t 
 end 
 
